michael_formal/types.thy
@@ -12,6 +12,7 @@ type_synonym update_function = "(string \<times> aexp) list"
 type_synonym statename = int
 type_synonym trace = "(label \<times> inputs) list" (*Ideally written as label(i1, i2, ...)*)
 type_synonym observation = "outputs list"
+type_synonym restriction = "(string \<times> bexp)"
 
 
 record transition =
